Array proof halfway done

timing/.Makefile.d
@@ -7,6 +7,12 @@ timing_auto.vos timing_auto.vok timing_auto.required_vos: timing_auto.v riscvTim
 memsolve.vo memsolve.glob memsolve.v.beautified memsolve.required_vo: memsolve.v riscvTiming.vo
 memsolve.vio: memsolve.v riscvTiming.vio
 memsolve.vos memsolve.vok memsolve.required_vos: memsolve.v riscvTiming.vos
-examples/RTOSDemo_NoAsserts_Clz.vo examples/RTOSDemo_NoAsserts_Clz.glob examples/RTOSDemo_NoAsserts_Clz.v.beautified examples/RTOSDemo_NoAsserts_Clz.required_vo: examples/RTOSDemo_NoAsserts_Clz.v 
-examples/RTOSDemo_NoAsserts_Clz.vio: examples/RTOSDemo_NoAsserts_Clz.v 
-examples/RTOSDemo_NoAsserts_Clz.vos examples/RTOSDemo_NoAsserts_Clz.vok examples/RTOSDemo_NoAsserts_Clz.required_vos: examples/RTOSDemo_NoAsserts_Clz.v 
+examples/FreeRTOS/RTOSDemo_NoAsserts_Clz.vo examples/FreeRTOS/RTOSDemo_NoAsserts_Clz.glob examples/FreeRTOS/RTOSDemo_NoAsserts_Clz.v.beautified examples/FreeRTOS/RTOSDemo_NoAsserts_Clz.required_vo: examples/FreeRTOS/RTOSDemo_NoAsserts_Clz.v 
+examples/FreeRTOS/RTOSDemo_NoAsserts_Clz.vio: examples/FreeRTOS/RTOSDemo_NoAsserts_Clz.v 
+examples/FreeRTOS/RTOSDemo_NoAsserts_Clz.vos examples/FreeRTOS/RTOSDemo_NoAsserts_Clz.vok examples/FreeRTOS/RTOSDemo_NoAsserts_Clz.required_vos: examples/FreeRTOS/RTOSDemo_NoAsserts_Clz.v 
+examples/data_structures/array.vo examples/data_structures/array.glob examples/data_structures/array.v.beautified examples/data_structures/array.required_vo: examples/data_structures/array.v ../Picinae_riscv.vo
+examples/data_structures/array.vio: examples/data_structures/array.v ../Picinae_riscv.vio
+examples/data_structures/array.vos examples/data_structures/array.vok examples/data_structures/array.required_vos: examples/data_structures/array.v ../Picinae_riscv.vos
+examples/data_structures/linked_list.vo examples/data_structures/linked_list.glob examples/data_structures/linked_list.v.beautified examples/data_structures/linked_list.required_vo: examples/data_structures/linked_list.v ../Picinae_riscv.vo
+examples/data_structures/linked_list.vio: examples/data_structures/linked_list.v ../Picinae_riscv.vio
+examples/data_structures/linked_list.vos examples/data_structures/linked_list.vok examples/data_structures/linked_list.required_vos: examples/data_structures/linked_list.v ../Picinae_riscv.vos
