timing/examples/data_structures/linked_list.c
@@ -1,0 +1,35 @@
+#include <stdint.h>
+#include <stddef.h>
+
+typedef struct list_node {
+   uint32_t value;
+   struct list_node* next;
+} list_node;
+
+void insert_after_pos_in_list(list_node* l, list_node* value, uint32_t position) {
+   if (l == NULL || value == NULL)
+	return;
+
+   for (uint32_t i = 0; i < position; i++) {
+       if (l->next == NULL)
+	       break;
+       l = l->next;
+   }
+   value->next = l->next;
+   l->next = value;
+}
+
+list_node* find_in_list(list_node* l, uint32_t key) {
+    if (l == NULL)
+	return NULL;
+
+    while (l != NULL) {
+    	if (l->value == key)
+	    return l;
+	l = l->next;
+    }
+
+    return NULL;
+}
+
+int main() {}
