timing/examples/data_structures/find_in_array.v
@@ -1,0 +1,200 @@
+Require Import array.
+Require Import riscvTiming.
+Import RISCVNotations.
+Require Import timing_auto.
+
+Variable ML : N.
+Variable ML_pos : 1 <= ML.
+
+Definition time_mem : N :=
+    5 + (ML - 2).
+Definition time_branch : N :=
+    5 + (ML - 1).
+
+Module find_in_arrayTime <: TimingModule.
+    Definition time_of_addr (s : store) (a : addr) : N :=
+        match neorv32_cycles_upper_bound ML s (array_bin a) with
+        | Some x => x | _ => 999 end.
+
+    Definition entry_addr : N := 0x101b0.
+
+    Definition exits (t:trace) : bool :=
+    match t with (Addr a,_)::_ => match a with
+    | 0x10214 => true
+    | _ => false
+  end | _ => false end.
+End find_in_arrayTime.
+
+Module find_in_arrayAuto := TimingAutomation find_in_arrayTime.
+Import find_in_arrayTime find_in_arrayAuto.
+
+Definition key_in_array (mem : addr -> N) (arr : addr) (key : N) : Prop :=
+    exists i, mem Ⓓ[arr + i] = key.
+
+Notation "'If' P 'Then' Q 'Else' R" := (
+    (P /\ Q) \/ (~P /\ R)
+) (at level 85).
+
+Definition mem_layout (sp : N) (arr : addr) (len : N) :=
+    create_noverlaps [(4, sp ⊖ 4); (4, sp ⊖ 8); 
+                      (4, sp ⊖ 20); (4, sp ⊖ 36); 
+                      (4, sp ⊖ 40); (4, sp ⊖ 44); 
+                      (4 * len, arr)].
+
+Definition time_of_find_in_array (mem : addr -> N) (arr : addr) (key : N) (len : N)
+        (t : trace) :=
+    If key_in_array mem arr key Then
+        cycle_count_of_trace t = 0
+    Else
+        cycle_count_of_trace t =
+            (* pre-loop time *)
+            4 + 10 * time_mem +
+            (* iterate len times *)
+            len *
+            (* full loop body length *)
+            (10 + (3 + (2/4) + (2 mod 4)) + time_mem + time_branch).
+
+Definition find_in_array_timing_invs (s : store) (base_mem : addr -> N)
+    (sp : N) (arr : addr) (key : N) (len : N) (t:trace) : option Prop :=
+match t with (Addr a, s) :: t' => match a with
+| 0x101b0 => Some (mem_layout sp arr len /\ s V_MEM32 = Ⓜbase_mem /\
+            s R_SP = Ⓓsp /\
+            s R_A0 = Ⓓarr /\ s R_A1 = Ⓓkey /\ s R_A2 = Ⓓlen /\
+            (key_in_array base_mem arr key \/ ~ key_in_array base_mem arr key) /\
+            cycle_count_of_trace t' = 0)
+| 0x101e0 => Some (mem_layout sp arr len /\ exists mem a5,
+    (* bindings *)
+    s R_S0 = Ⓓsp /\ s R_A2 = Ⓓlen /\ s R_A4 = Ⓓarr /\
+    s R_A5 = Ⓓa5 /\ s V_MEM32 = Ⓜmem /\
+    (* preservation *)
+    (forall i, i < len ->
+        mem Ⓓ[arr + i] = base_mem Ⓓ[arr + i]) /\
+    (key_in_array base_mem arr key \/ ~ key_in_array base_mem arr key) /\
+    mem Ⓓ[sp ⊖ 20] <= len /\
+    cycle_count_of_trace t' =
+        (* pre-loop time *)
+        4 + 10 * time_mem +
+        (* loop counter stored in register a5 *)
+        a5 *
+        (* full loop body length - can't have broken out by this address *)
+        (10 + (3 + (2/4) + (2 mod 4)) + time_mem + time_branch)
+    )
+| 0x10214 => Some (time_of_find_in_array base_mem arr key len t)
+| _ => None end | _ => None end.
+
+Definition lifted_find_in_array : program :=
+    lift_riscv array_bin.
+
+(* We use simpl in a few convenient places: make sure it doesn't go haywire *)
+Arguments N.add _ _ : simpl nomatch.
+Arguments N.mul _ _ : simpl nomatch.
+
+Ltac fold_big_subs :=
+    repeat match goal with
+    | [ |- context[?M [Ⓓ ?X + ?B + ?N := ?V]] ] =>
+      rewrite <-(setmem_mod_l _ _ _ M (X+B+N) V);
+      replace (M [ⒹX+B⊕N := V]) with
+        (M [Ⓓ(msub 32 B (2^32 - X)) ⊕ N := V]) by
+        (unfold msub; now psimpl);
+      simpl (2^32 - X)
+    | [ |- context[?M [Ⓓ?X + ?Y := ?V]]] =>
+      rewrite <- setmem_mod_l with (a := X + Y);
+      replace (X⊕Y) with (msub 32 Y (2^32 - X)) by (now rewrite N.add_comm);
+      simpl (2^32 - X)
+    | [ |- context[?M Ⓓ[ ?X + ?B + ?N]] ] =>
+      rewrite <-(getmem_mod_l _ _ _ M (X+B+N));
+      replace (M Ⓓ[X+B⊕N]) with
+        (M Ⓓ[(msub 32 B (2^32 - X)) ⊕ N]) by
+        (unfold msub; now psimpl);
+      simpl (2^32 - X)
+    | [ |- context[?M Ⓓ[?X + ?Y]]] =>
+      rewrite <- getmem_mod_l with (a := X + Y);
+      replace (X⊕Y) with (msub 32 Y (2^32 - X)) by (now rewrite N.add_comm);
+      simpl (2^32 - X)
+    end.
+
+Theorem find_in_array_timing:
+  forall s t s' x' base_mem sp arr key len
+         (ENTRY: startof t (x',s') = (Addr entry_addr, s))
+         (MDL: models rvtypctx s)
+         (MEM: s V_MEM32 = Ⓜbase_mem)
+         (SP: s R_SP = Ⓓsp)
+         (A0: s R_A0 = Ⓓarr)
+         (A1: s R_A1 = Ⓓkey)
+         (A2: s R_A2 = Ⓓlen)
+         (IN: key_in_array base_mem arr key \/ ~ key_in_array base_mem arr key)
+         (MEMLAYOUT: mem_layout sp arr len),
+  satisfies_all 
+    lifted_find_in_array
+    (find_in_array_timing_invs s base_mem sp arr key len)
+    exits
+  ((x',s')::t).
+Proof using.
+    intros.
+    apply prove_invs.
+    Local Ltac step := time rv_step.
+
+    simpl. rewrite ENTRY. unfold entry_addr. step.
+    split. unfold mem_layout in *. noverlaps_preserved idtac.
+    now repeat split.
+
+    intros.
+    eapply startof_prefix in ENTRY; try eassumption.
+    eapply preservation_exec_prog in MDL; 
+        try eassumption; [idtac|apply lift_riscv_welltyped].
+    clear - ENTRY PRE MDL. rename t1 into t. rename s1 into s'.
+
+    destruct_inv 32 PRE.
+
+    destruct PRE as (Layout & Mem & SP & A0 & A1 & A2 & IN & Cycles).
+    repeat step.
+        split. unfold mem_layout in *. noverlaps_preserved idtac. 
+        repeat eexists.
+        intros.
+            unfold mem_layout in *. unfold_create_noverlaps.
+            fold_big_subs.
+            repeat rewrite getmem_noverlap. reflexivity.
+            1-6:
+                eapply noverlap_shrink with (a1 := arr) (len1 := 4 * len);
+                auto using noverlap_symmetry;
+                psimpl; rewrite N.mod_small; try lia; transitivity len;
+                try assumption; apply (rv_regsize MDL A2).
+        assumption. psimpl. lia.
+        hammer. find_rewrites. unfold time_mem, time_branch.
+        lia.
+
+    destruct PRE as (Layout & mem & a5 & S0 & A2 & A4 & A5 & MEM & Preserved & 
+        IN & LEN & Cycles).
+    destruct IN.
+    (* There is a matching element in the array *) {
+        step.
+        repeat step.
+        (* postcondition after loop condition fail *)
+            unfold time_of_find_in_array. left.
+            split. assumption. admit.
+        (* loop invariant after going around *)
+            split. unfold mem_layout in *. noverlaps_preserved idtac.
+            repeat eexists; auto.
+            hammer. find_rewrites.
+            unfold time_mem, time_branch. psimpl.
+            change (2/4) with 0.
+            rewrite N.mod_small. lia.
+                apply Bool.negb_false_iff, N.ltb_lt in BC.
+                apply N.le_lt_trans with len.
+                lia.
+                apply (rv_regsize MDL A2).
+        (* postcondition after loop break *)
+        repeat step.
+            unfold time_of_find_in_array. left.
+            split. assumption. admit.
+    }
+
+    (* There is not a matching element in the array *) {
+        step.
+        do 4 step.
+        (* contradiction - BC0 says a match has been found *)
+            exfalso. apply H. exists a5.
+            rewrite <- Preserved.
+    }
+Qed.
+
